PHAxioms.v
@@ -1,6 +1,7 @@
 Set Implicit Arguments.
 
 Require Import Relation.
+Require Import Packet.
 Require Import Omega.
 Require Import Syntax.
 Require Import Semantics.
@@ -9,28 +10,21 @@ Require Import Coq.Classes.Equivalence.
 Require Import Coq.Arith.EqNat.
 Require Import Coq.Logic.FunctionalExtensionality.
 Require Import Coq.Setoids.Setoid.
+Require Import Coq.Program.Equality.
 
  Existing Instances Equivalence_exp.
  Local Open Scope equiv_scope.
- 
- Lemma PA_Mod_Mod_Comm_Help: 
-   forall (f1 f2 : field) (x : packet) (n1 n2 : nat), ~(f1 = f2) ->
-   set_field_p (set_field_p x f1 n1) f2 n2 = set_field_p (set_field_p x f2 n2) f1 n1.
- Proof with auto.
-   intros. destruct x. 
-   destruct f1; destruct f2; try solve [simpl; auto | contradiction H; auto]. 
- Qed.  
 
  Lemma PA_Mod_Mod_Comm_Help2:
-   forall (f1 f2 : field) (x : history) (n1 n2 : nat), ~(f1 = f2) ->
+   forall (f1 f2 : field) (x : history) (n1 n2 : val), ~(f1 = f2) ->
      set_field (set_field x f1 n1) f2 n2 = set_field (set_field x f2 n2) f1 n1.
  Proof with auto.
    intros.
-   destruct x; simpl; rewrite -> PA_Mod_Mod_Comm_Help...
+   destruct x; simpl; rewrite -> Packet.mod_mod_comm...
  Qed.
       
  Lemma PA_Mod_Mod_Comm:
-   forall (f1 f2 : field) (n1 n2 : nat), ~(f1 = f2) -> 
+   forall (f1 f2 : field) (n1 n2 : val), ~(f1 = f2) -> 
     (Seq (Mod f1 n1) (Mod f2 n2)) 
      === (Seq (Mod f2 n2) (Mod f1 n1)).
  Proof with auto.
@@ -40,9 +34,9 @@ Require Import Coq.Setoids.Setoid.
  Qed.
 
  Lemma set_other_field_not_effect:
-   forall (f1 f2 : field) (n1 n2 : nat) (x : history), ~(f1 = f2) ->
-     (get_Field (get_Packet (set_field x f1 n1)) f2) =
-     (get_Field (get_Packet x) f2).
+   forall (f1 f2 : field) (n1 n2 : val) (x : history), ~(f1 = f2) ->
+     (Packet.get_field f2 (get_packet (set_field x f1 n1))) =
+     (Packet.get_field f2 (get_packet x)).
    Proof with auto.
      intros. destruct x. destruct p.
      + destruct f1; destruct f2; simpl; auto; try solve [contradiction H; auto].
@@ -50,87 +44,89 @@ Require Import Coq.Setoids.Setoid.
    Qed.
     
  Lemma PA_Mod_Filter_Comm:
-   forall (f1 f2 : field) (n1 n2 : nat), ~(f1 = f2) ->
+   forall (f1 f2 : field) (n1 n2 : val), ~(f1 = f2) ->
      (Seq (Mod f1 n1) (Match f2 n2)) === (Seq (Match f2 n2) (Mod f1 n1)).
  Proof with auto.
-   intros. split; intros; simpl in *; unfold join in *; destruct H0 as [z [H1 H2]]; subst.
-     remember (beq_nat (get_Field (get_Packet (set_field x f1 n1)) f2) n2).
-     destruct b... subst. exists x. split... subst. 
-     rewrite set_other_field_not_effect in Heqb. rewrite <- Heqb...
-     trivial. trivial. contradiction.
+   intros. split ; intros; simpl in *; unfold join in *; destruct H0 as [z [H1 H2]]; subst.
+     remember (Packet.beq_val (Packet.get_field f2 (get_packet (set_field x f1 n1))) n2).
+     destruct b... subst. exists x. split...
+     + rewrite set_other_field_not_effect in Heqb.
+       remember (Packet.beq_val (Packet.get_field f2 (get_packet x)) n2).
+       destruct b. reflexivity. inversion Heqb. trivial. trivial. 
+   + contradiction. 
    + rewrite <- set_other_field_not_effect with (f1 := f1) (n1 := n1) in H1...
-     remember (beq_nat (get_Field (get_Packet (set_field x f1 n1)) f2) n2).
+     remember (Packet.beq_val (Packet.get_field f2 (get_packet (set_field x f1 n1))) n2).
      destruct b. subst. exists (set_field z f1 n1). split... rewrite <- Heqb...
      contradiction.
  Qed.
 
  Lemma obs_doesnt_matter:
-   forall (f1 : field) (n1 : nat) (x : history),
-     (get_Field (get_Packet (ConsHist (get_Packet x) x)) f1) = 
-     (get_Field (get_Packet x) f1).
+   forall (f1 : field) (n1 : val) (x : history),
+     (Packet.get_field f1 (get_packet (ConsHist (get_packet x) x))) = 
+     (Packet.get_field f1 (get_packet x)).
    Proof.
      intros. auto.
  Qed.
 
  Lemma PA_Obs_Filter_Comm:
-   forall (f1 : field) (n1 : nat),
+   forall (f1 : field) (n1 : val),
      (Seq Obs (Match f1 n1)) === (Seq (Match f1 n1) Obs).
  Proof with auto.
    intros. split; intros; simpl in *; unfold join in *; destruct H as [z [H0 H1]]; subst. 
    + exists x.
-    remember (beq_nat (get_Field (get_Packet (ConsHist (get_Packet x) x)) f1) n1).
+    remember (Packet.beq_val (Packet.get_field f1 (get_packet (ConsHist (get_packet x) x))) n1).
      destruct b. split... rewrite obs_doesnt_matter in Heqb. rewrite <- Heqb... trivial.
     contradiction.
-   + exists (ConsHist (get_Packet x) x). split...
+   + exists (ConsHist (get_packet x) x). split...
      rewrite <- obs_doesnt_matter in H0.
-     remember (beq_nat (get_Field (get_Packet (ConsHist (get_Packet x) x)) f1) n1).
+     remember (Packet.beq_val (Packet.get_field f1 (get_packet (ConsHist (get_packet x) x))) n1).
      destruct b. subst... contradiction. trivial.
  Qed.
   
   Lemma always_true:
-    forall (f1 : field) (n1 : nat) (x : history), 
-     beq_nat (get_Field (get_Packet (set_field x f1 n1)) f1) n1 = true.
+    forall (f1 : field) (n1 : val) (x : history), 
+     Packet.beq_val (Packet.get_field f1 (get_packet (set_field x f1 n1))) n1 = true.
   Proof with auto.
-    intros. destruct x; destruct p; simpl; unfold set_field_p; simpl; destruct f1;
-    simpl; induction n1... 
+    intros; assert (true = Packet.beq_val n1 n1). rewrite Packet.beq_val_means with (v1 := n1) (v2 := n1); reflexivity.
+    destruct x; destruct p; simpl; unfold Packet.set_field; simpl; destruct f1; simpl; rewrite H; reflexivity.
  Qed.
 
   Lemma PA_Mod_Filter:
-    forall (f1 : field) (n1 : nat),
+    forall (f1 : field) (n1 : val),
       (Seq (Mod f1 n1) (Match f1 n1)) === (Mod f1 n1).
   Proof with auto.
     intros. split; intros; simpl in *; unfold join in *.
     + destruct H as [z [h1 h2]].
-      subst. remember (beq_nat (get_Field (get_Packet (set_field x f1 n1)) f1) n1).
+      subst. remember (Packet.beq_val (Packet.get_field f1 (get_packet (set_field x f1 n1))) n1).
       destruct b. subst... contradiction.
     + subst. exists (set_field x f1 n1).
       split... rewrite always_true...
   Qed.
   
   Lemma Mod_to_Filter: 
-    forall (f1 : field) (n1 : nat) (z : history), 
-      (get_Field (get_Packet z) f1) = n1 -> z = set_field z f1 n1.
+    forall (f1 : field) (n1 : val) (z : history), 
+      (Packet.get_field f1 (get_packet z)) = n1 -> z = set_field z f1 n1.
   Proof with auto.
     intros. destruct z; destruct p; simpl; destruct f1; simpl in *; subst...
   Qed.
 
   Lemma PA_Filter_Mod:
-    forall (f1 : field) (n1 : nat), 
+    forall (f1 : field) (n1 : val), 
       (Seq (Match f1 n1) (Mod f1 n1)) === (Match f1 n1).
   Proof with auto with arith.
     intros. split; intros; simpl in *; unfold join in *.
     + destruct H as [z [H1 H2]].
-      subst. remember (beq_nat (get_Field (get_Packet x) f1) n1).
-      destruct b. subst. apply Mod_to_Filter. apply beq_nat_eq in Heqb...
+      subst. remember (Packet.beq_val (Packet.get_field f1 (get_packet x)) n1).
+      destruct b. subst. apply Mod_to_Filter. apply Packet.beq_val_means in Heqb...
       contradiction.
     + exists y. split...
-      remember (beq_nat (get_Field (get_Packet x) f1) n1).
-      destruct b. subst. apply beq_nat_eq in Heqb. apply Mod_to_Filter in Heqb...
+      remember (Packet.beq_val (Packet.get_field f1 (get_packet x)) n1).
+      destruct b. subst. apply Packet.beq_val_means in Heqb. apply Mod_to_Filter in Heqb...
       contradiction.
   Qed. 
 
   Lemma PA_Mod_Mod:
-    forall (f1 : field) (n1 n2: nat), 
+    forall (f1 : field) (n1 n2: val), 
       (Seq (Mod f1 n1) (Mod f1 n2)) === (Mod f1 n2).
   Proof with auto.
     intros. split; intros; simpl in *; unfold join in *.
@@ -141,15 +137,15 @@ Require Import Coq.Setoids.Setoid.
   Qed.
       
   Lemma PA_Contra:
-    forall (f1 : field) (n1 n2 : nat), (n1 <> n2) ->
+    forall (f1 : field) (n1 n2 : val), (n1 <> n2) ->
       (Seq (Match f1 n1) (Match f1 n2)) === Drop.
   Proof with auto.
     intros. split; intros; simpl in *; unfold join in *.
     + destruct H0 as [z [H0 H1]]. unfold empty.
-      remember (beq_nat (get_Field (get_Packet x) f1) n1).
-      remember (beq_nat (get_Field (get_Packet z) f1) n2).
+      remember (Packet.beq_val (Packet.get_field f1 (get_packet x)) n1).
+      remember (Packet.beq_val (Packet.get_field f1 (get_packet z)) n2).
       destruct b; destruct b0; subst; destruct y; simpl in *; 
-      destruct p; try solve [apply beq_nat_eq in Heqb; apply beq_nat_eq in Heqb0;
+      destruct p; try solve [apply Packet.beq_val_means in Heqb; apply Packet.beq_val_means in Heqb0;
       subst; destruct f1; contradiction H; auto]; contradiction.
     + unfold empty in H0. contradiction.
   Qed.
